Test/civl/samples/two-lists.bpl
@@ -1,0 +1,134 @@
+// RUN: %parallel-boogie -lib:base -lib:node -vcsSplitOnEveryAssert "%s" > "%t"
+// RUN: %diff "%s.expect" "%t"
+
+type ListElem T = Node Loc T;
+
+datatype Queue<T> { Queue(head: Loc, tail: Loc, {:linear} nodes: Map Loc (ListElem T)) }
+
+var {:linear} {:layer 0, 1} lists: Map Loc (Queue int);
+
+var {:linear} {:layer 0, 1} pos: One (TaggedLoc Unit);
+var {:linear} {:layer 0, 1} neg: One (TaggedLoc Unit);
+
+yield procedure {:layer 0} ReadPos() returns (loc: Loc);
+refines both action {:layer 1} _ {
+    loc := pos->val->loc;
+}
+
+yield procedure {:layer 0} ReadNeg() returns (loc: Loc);
+refines both action {:layer 1} _ {
+    loc := neg->val->loc;
+}
+
+yield procedure {:layer 0} Enqueue(loc_q: Loc, i: int);
+refines action {:layer 1} _
+{
+    var {:linear} one_loc_q: One Loc;
+    var {:linear} queue: Queue int;
+    var head, tail: Loc;
+    var {:linear} nodes: Map Loc (ListElem int);
+    var {:linear} one_loc_n, new_one_loc_n: One Loc;
+    var node: ListElem int;
+
+    call one_loc_q, queue := Map_Get(lists, loc_q);
+    Queue(head, tail, nodes) := queue;
+
+    call new_one_loc_n := Loc_New();
+    call Map_Put(nodes, new_one_loc_n, Node(None(), 0));
+
+    call one_loc_n, node := Map_Get(nodes, tail);
+    node := Node(Some(new_one_loc_n->val), i);
+    call Map_Put(nodes, one_loc_n, node);
+
+    queue := Queue(head, new_one_loc_n->val, nodes);
+    call Map_Put(lists, one_loc_q, queue);
+}
+
+yield procedure {:layer 0} Dequeue(loc_q: Loc) returns (i: int);
+refines action {:layer 1} _
+{
+    var {:linear} one_loc_q: One Loc;
+    var {:linear} queue: Queue int;
+    var head, tail: Loc;
+    var {:linear} nodes: Map Loc (ListElem int);
+    var {:linear} one_loc_n: One Loc;
+    var node: ListElem int;
+    var next: Option Loc;
+
+    call one_loc_q, queue := Map_Get(lists, loc_q);
+    Queue(head, tail, nodes) := queue;
+    
+    assume head != tail;
+    call one_loc_n, node := Map_Get(nodes, head);
+    Node(next, i) := node;
+
+    assert next is Some;
+    queue := Queue(next->t, tail, nodes);
+    call Map_Put(lists, one_loc_q, queue);
+}
+
+
+function {:inline} IsAcyclic(q: Queue int): bool
+{
+    Between(q->nodes->val, Some(q->head), Some(q->tail), None())
+}
+
+function {:inline} QueueElems(q: Queue int): [Loc]bool 
+{
+    BetweenSet(q->nodes->val, Some(q->head), Some(q->tail))
+}
+
+yield invariant {:layer 1} PosInv();
+invariant Map_Contains(lists, pos->val->loc);
+invariant (var q := Map_At(lists, pos->val->loc); IsAcyclic(q) &&
+            (forall loc_n: Loc:: QueueElems(q)[loc_n] ==>
+                Map_Contains(q->nodes, loc_n) &&
+                (loc_n == q->tail || (var node := Map_At(q->nodes, loc_n); node->val > 0))));
+
+yield invariant {:layer 1} NegInv();
+invariant Map_Contains(lists, neg->val->loc);
+invariant (var q := Map_At(lists, neg->val->loc); IsAcyclic(q) &&
+            (forall loc_n: Loc:: QueueElems(q)[loc_n] ==>
+                Map_Contains(q->nodes, loc_n) &&
+                (loc_n == q->tail || (var node := Map_At(q->nodes, loc_n); node->val < 0))));
+
+
+yield procedure {:layer 1} Producer(i: int)
+preserves call PosInv();
+preserves call NegInv();
+{
+    var loc: Loc;
+
+    assert {:layer 1} pos->val->loc != neg->val->loc;
+    if (i == 0) {
+        return;
+    }
+    if (i > 0) {
+        call loc := ReadPos();
+    } else {
+        call loc := ReadNeg();
+    }
+    call Enqueue(loc, i);
+}
+
+yield procedure {:layer 1} PosConsumer()
+preserves call PosInv();
+{
+    var loc: Loc;
+    var i: int;
+
+    call loc := ReadPos();
+    call i := Dequeue(loc);
+    assert {:layer 1} i > 0;
+}
+
+yield procedure {:layer 1} NegConsumer()
+preserves call NegInv();
+{
+    var loc: Loc;
+    var i: int;
+
+    call loc := ReadNeg();
+    call i := Dequeue(loc);
+    assert {:layer 1} i < 0;
+}
